Got to the substitution lemma (work in progress)

examples/metatheory/stlc_constr_db.fst
@@ -39,6 +39,10 @@ let rec subst e s =
   | EAbs t e1 -> EAbs t (subst e1 (fun x -> if x = 0 then EVar x else s (x+1)))
   | EApp e1 e2 -> EApp (subst e1 s) (subst e2 s)
 
+val subst_beta : exp -> exp -> Tot exp
+let subst_beta v e =
+  subst e (fun x -> if x = 0 then v else EVar (x-1))
+
 val step : exp -> Tot (option exp)
 let rec step e =
   match e with
@@ -46,7 +50,7 @@ let rec step e =
       if is_value e1 then
         if is_value e2 then
           match e1 with
-          | EAbs t e' -> Some (subst e' (fun x -> if x = 0 then e2 else EVar (x-1)))
+          | EAbs t e' -> Some (subst_beta e' e2)
           | _         -> None
         else
           match (step e2) with
@@ -93,36 +97,34 @@ let rec progress _ _ h =
   | TyAbs _ _ -> ()
   | TyApp h1 h2 -> progress h1; progress h2
 
-(* variable 
-val appears_free_in : x:nat -> e:exp -> l:nat -> Tot bool
+val appears_free_in : x:var -> e:exp -> Tot bool (decreases e)
 let rec appears_free_in x e =
   match e with
   | EVar y -> x = y
   | EApp e1 e2 -> appears_free_in x e1 || appears_free_in x e2
-  | EAbs y _ e1 -> x <> y && appears_free_in x e1
+  | EAbs _ e1 -> appears_free_in (x+1) e1
 
-(*
-val free_in_context : x:int -> #e:exp -> #g:env -> #t:ty -> h:rtyping g e t ->
+val free_in_context : x:var -> #e:exp -> #g:env -> #t:ty -> h:rtyping g e t ->
       Lemma (ensures (appears_free_in x e ==> is_Some (g x))) (decreases h)
 let rec free_in_context x _ _ _ h =
   match h with
   | TyVar x -> ()
-  | TyAbs y t h1 -> free_in_context x h1
+  | TyAbs t h1 -> free_in_context (x+1) h1
   | TyApp h1 h2 -> free_in_context x h1; free_in_context x h2
 
-val typable_empty_closed : x:int -> #e:exp -> #t:ty -> rtyping empty e t ->
+val typable_empty_closed : x:var -> #e:exp -> #t:ty -> rtyping empty e t ->
       Lemma (ensures (not(appears_free_in x e)))
 (*      [SMTPat (appears_free_in x e)] -- CH: adding this makes it fail! *)
 let typable_empty_closed x _ _ h = free_in_context x h
 
 val typable_empty_closed' : #e:exp -> #t:ty -> rtyping empty e t ->
-      Lemma (ensures (forall (x:int). (not(appears_free_in x e))))
+      Lemma (ensures (forall (x:var). (not(appears_free_in x e))))
 let typable_empty_closed' _ _ h = admit() (* CH: need forall_intro for showing this *)
 
 opaque logic type Equal (g1:env) (g2:env) =
-                 (forall (x:int). g1 x=g2 x)
+                 (forall (x:var). g1 x=g2 x)
 opaque logic type EqualE (e:exp) (g1:env) (g2:env) =
-                 (forall (x:int). appears_free_in x e ==> g1 x=g2 x)
+                 (forall (x:var). appears_free_in x e ==> g1 x=g2 x)
 
 val context_invariance : #e:exp -> #g:env -> #t:ty -> 
       h:(rtyping g e t) -> g':env{EqualE e g g'} ->
@@ -130,8 +132,8 @@ val context_invariance : #e:exp -> #g:env -> #t:ty ->
 let rec context_invariance _ _ _ h g' =
   match h with
   | TyVar x -> TyVar x
-  | TyAbs y t_y h1 ->
-    TyAbs y t_y (context_invariance h1 (extend g' y t_y))
+  | TyAbs t_y h1 ->
+    TyAbs t_y (context_invariance h1 (extend g' t_y))
   | TyApp h1 h2 ->
     TyApp (context_invariance h1 g') (context_invariance h2 g')
 
@@ -140,30 +142,76 @@ val typing_extensional : #e:exp -> #g:env -> #t:ty ->
       Tot (rtyping g' e t)
 let typing_extensional _ _ _ h g' = context_invariance h g'
 
-(* CH: would it be possible to prove this with x implicit? maybe not ... *)
+assume val admit: unit -> Pure 'a (requires True) (ensures (fun _ -> False))
+
+val subst_gen : var -> exp -> exp -> Tot exp
+let subst_gen x v e =
+  subst e (fun y -> if y < x then (EVar y)
+                    else if y = x then v
+                    else (EVar (y-1+x)))
+
+(* Proof of this will probably rely on an extensionality property of subst *)
+val subst_beta_gen : v:exp -> e:exp -> Lemma 
+  (ensures (subst_beta v e = subst_gen 0 v e)) (decreases e)
+let subst_beta_gen v e =
+  match e with
+  | EVar _ -> admit()
+  | EAbs _ _ -> admit()
+  | EApp _ _  -> admit()
+
+val subst_gen_var_eq : x:var -> v:exp -> Lemma
+  (ensures (subst_gen x v (EVar x) = v))
+let subst_gen_var_eq x v = admit()
+
+val subst_gen_var_neq : x:var -> y:var -> v:exp -> Lemma
+  (ensures (subst_gen x v (EVar y) = (EVar y)))
+let subst_gen_var_neq x y v = admit()
+
+val extend_gen : var -> env -> ty -> Tot env
+let extend_gen x g t y = if y < x then g y 
+                         else if y = x then Some t
+                         else g (y-1)
+
 val substitution_preserves_typing :
-      x:int -> #e:exp -> #v:exp -> #t_x:ty -> #t:ty -> #g:env ->
+      x:var -> #e:exp -> #v:exp -> #t_x:ty -> #t:ty -> #g:env ->
       h1:rtyping empty v t_x ->
-      h2:rtyping (extend g x t_x) e t ->
-      Tot (rtyping g (subst x v e) t) (decreases e)
-let rec substitution_preserves_typing x _ v t_x t g h1 h2 =
+      h2:rtyping (extend_gen x g t_x) e t ->
+      Tot (rtyping g (subst_gen x v e) t) (decreases e)
+let rec substitution_preserves_typing x e v t_x t g h1 h2 =
   match h2 with
   | TyVar y ->
      if x=y
-     then (typable_empty_closed' h1; context_invariance h1 g)
-     else context_invariance h2 g
-  | TyAbs y t_y h21 ->
-     let gy = extend g y t_y in
-     if x=y
-     then TyAbs y t_y (typing_extensional h21 gy)
+     then (typable_empty_closed' h1;
+           subst_gen_var_eq x v;
+           context_invariance h1 g)
+     else (subst_gen_var_neq x y v;
+           (*assert(EqualE e (extend_gen x g t_x) g);
+             -- this assert fails, so we can't call context_invariance *)
+           admit() (*context_invariance h2 g*))
+  | TyAbs t_y h21 -> admit()
+(*
+     let gy = extend g t_y in
+     if x=0
+     then TyAbs t_y (typing_extensional h21 gy)
      else
-       (let h21' = typing_extensional h21 (extend gy x t_x) in
-        TyAbs y t_y (substitution_preserves_typing x h1 h21'))
-  | TyApp #g' #e1 #e2 #t11 #t12 h21 h22 -> (* CH: implicits don't work here, why? *)
-     TyApp #g #(subst x v e1) #(subst x v e2) #t11 #t12
+       (let h21' = typing_extensional h21 (extend gy t_x) in
+        TyAbs t_y (substitution_preserves_typing x h1 h21'))
+*)
+  | TyApp #g' #e1 #e2 #t11 #t12 h21 h22 -> admit()
+(*
+     (* CH: implicits don't work here, why? *)
+     TyApp #g #(subst_gen x v e1) #(subst_gen x v e2) #t11 #t12
        (substitution_preserves_typing x h1 h21)
        (substitution_preserves_typing x h1 h22)
+*)
 
+assume val subst_beta_preserves_typing :
+      #e:exp -> #v:exp -> #t_x:ty -> #t:ty -> #g:env ->
+      h1:rtyping empty v t_x ->
+      h2:rtyping (extend g t_x) e t ->
+      Tot (rtyping g (subst_beta v e) t) (decreases e)
+
+(*
 val preservation : #e:exp{is_Some (step e)} -> #t:ty -> h:(rtyping empty e t) ->
       Tot (rtyping empty (Some.v (step e)) t) (decreases e)
 let rec preservation e t h =
